# baseURI: http://www.w3.org/ns/project
# imports: http://purl.org/dc/elements/1.1/
# imports: http://www.w3.org/ns/prov-o#
# prefix: proj

@prefix dc: <http://purl.org/dc/elements/1.1/> .
@prefix dcterms: <http://purl.org/dc/terms/> .
@prefix owl: <http://www.w3.org/2002/07/owl#> .
@prefix proj: <http://www.w3.org/ns/project#> .
@prefix proji: <http://www.w3.org/ns/project/> .
@prefix prov: <http://www.w3.org/ns/prov#> .
@prefix rdf: <http://www.w3.org/1999/02/22-rdf-syntax-ns#> .
@prefix rdfs: <http://www.w3.org/2000/01/rdf-schema#> .
@prefix skos: <http://www.w3.org/2004/02/skos/core#> .
@prefix voaf: <http://purl.org/vocommons/voaf#> .
@prefix xsd: <http://www.w3.org/2001/XMLSchema#> .

<http://www.w3.org/ns/project>
  rdf:type owl:Ontology ;
  dc:contributor "Peter BRENTON, CSIRO" ;
  dc:creator "Simon J D COX, CSIRO" ;
  dcterms:created "2017-08-14"^^xsd:date ;
  dcterms:creator <http://orcid.org/0000-0002-3884-3420> ;
  dcterms:license <https://creativecommons.org/licenses/by/4.0/> ;
  voaf:exampleDataset <https://raw.githubusercontent.com/dr-shorthair/ont/gh-pages/project/examples.ttl> ;
  voaf:extends <http://www.w3.org/ns/prov-o> ;
  voaf:reliesOn <http://www.w3.org/2004/02/skos/core> ;
  rdfs:comment """A basic ontology for projects, influenced by FOAF, dbPedia, VIVO-ISF, but only depending on W3C PROV-O.

Can be used for alignment of project related classes and properties in more specific applications.""" ;
  rdfs:comment """TODO:
1. figure out how to link to prov:Plan""" ;
  owl:imports dc: ;
  owl:imports <http://www.w3.org/ns/prov-o#> ;
.
proj:FundingAssociation
  rdf:type owl:Class ;
  rdfs:label "Funding association" ;
  rdfs:subClassOf prov:Association ;
  rdfs:subClassOf [
      rdf:type owl:Restriction ;
      owl:hasValue proji:Funder ;
      owl:onProperty prov:hadRole ;
    ] ;
  rdfs:subClassOf [
      rdf:type owl:Restriction ;
      owl:minCardinality "1"^^xsd:nonNegativeInteger ;
      owl:onProperty proj:fundsProvided ;
    ] ;
.
proj:Project
  rdf:type owl:Class ;
  rdfs:comment """Basic project class.

A Project is an activity with a budget, a sponsor, and a leader. It has planned start and end dates, which may differ from the actuals.

Project stakeholders are indicated using the prov:qualifiedAssociation structure which allows their role to be catpured. Some special stakeholders have specific sub-properties with the roles fixed, including project-leader, project-participant, and project-funder.

Activities within a project are indicated using the hasSubActivity (simple) or subActivityAssociation properties - the latter allowing the nature of the relationshp to be described as well. """ ;
  rdfs:label "Project" ;
  rdfs:subClassOf prov:Activity ;
  rdfs:subClassOf [
      rdf:type owl:Restriction ;
      owl:cardinality "1"^^xsd:nonNegativeInteger ;
      owl:onProperty proj:hadBudgetTotal ;
    ] ;
  rdfs:subClassOf [
      rdf:type owl:Restriction ;
      owl:cardinality "1"^^xsd:nonNegativeInteger ;
      owl:onProperty proj:plannedEndTime ;
    ] ;
  rdfs:subClassOf [
      rdf:type owl:Restriction ;
      owl:cardinality "1"^^xsd:nonNegativeInteger ;
      owl:onProperty proj:plannedStartTime ;
    ] ;
  rdfs:subClassOf [
      rdf:type owl:Restriction ;
      owl:minCardinality "1"^^xsd:nonNegativeInteger ;
      owl:onProperty proj:hadLeader ;
    ] ;
  rdfs:subClassOf [
      rdf:type owl:Restriction ;
      owl:minCardinality "1"^^xsd:nonNegativeInteger ;
      owl:onProperty proj:hasSponsor ;
    ] ;
.
proj:ResearchProject
  rdf:type owl:Class ;
  rdfs:comment "A research project has one or more PIs who are individual persons, and should be classified according to standard research classification such as the Australian Bureau of Statistics ANZSRC-FOR or NASA's Global Change Master Directory - Science Keywords." ;
  rdfs:label "Research Project" ;
  rdfs:subClassOf proj:Project ;
  rdfs:subClassOf [
      rdf:type owl:Restriction ;
      owl:minCardinality "1"^^xsd:nonNegativeInteger ;
      owl:onProperty proj:hadFieldOfResearch ;
    ] ;
.
proj:SumOfMoney
  rdf:type owl:Class ;
  rdfs:label "Amount of money" ;
  rdfs:subClassOf [
      rdf:type owl:Restriction ;
      owl:cardinality "1"^^xsd:nonNegativeInteger ;
      owl:onProperty proj:moneyAmount ;
    ] ;
  rdfs:subClassOf [
      rdf:type owl:Restriction ;
      owl:cardinality "1"^^xsd:nonNegativeInteger ;
      owl:onProperty proj:moneyCurrency ;
    ] ;
.
proj:fundsProvided
  rdf:type owl:ObjectProperty ;
  rdfs:label "funding provided" ;
  rdfs:range proj:SumOfMoney ;
.
proj:grantNumber
  rdf:type owl:AnnotationProperty ;
  rdfs:domain proj:FundingAssociation ;
  rdfs:label "Funder's grant number" ;
  rdfs:range xsd:string ;
.
proj:hadAreaOfInterest
  rdf:type owl:ObjectProperty ;
  rdfs:comment "The name and label of this property are phrased retrospectively (had, was) which is consistent with PROV-O, but may be used for a contemporary relationship (has, is) while the project is underway." ;
  rdfs:comment "address, place, locality, location, etc" ;
  rdfs:domain proj:Project ;
  rdfs:label "has area of interest" ;
  rdfs:subPropertyOf prov:atLocation ;
.
proj:hadBudgetTotal
  rdf:type owl:ObjectProperty ;
  rdfs:comment "The name and label of this property are phrased retrospectively (had, was) which is consistent with PROV-O, but may be used for a contemporary relationship (has, is) while the project is underway." ;
  rdfs:domain proj:Project ;
  rdfs:label "total budget" ;
  rdfs:range proj:SumOfMoney ;
.
proj:hadFieldOfResearch
  rdf:type owl:ObjectProperty ;
  rdfs:comment "The name and label of this property are phrased retrospectively (had, was) which is consistent with PROV-O, but may be used for a contemporary relationship (has, is) while the project is underway." ;
  rdfs:domain proj:ResearchProject ;
  rdfs:label "field of research" ;
  rdfs:range skos:Concept ;
  rdfs:subPropertyOf dcterms:subject ;
.
proj:hadLeader
  rdf:type owl:ObjectProperty ;
  rdfs:comment "The name and label of this property are phrased retrospectively (had, was) which is consistent with PROV-O, but may be used for a contemporary relationship (has, is) while the project is underway." ;
  rdfs:domain prov:Activity ;
  rdfs:label "activity leader" ;
  rdfs:range prov:Person ;
  rdfs:subPropertyOf prov:wasAssociatedWith ;
  owl:propertyChainAxiom (
      [
        rdf:type owl:ObjectProperty ;
        rdfs:range [
            rdf:type owl:Class ;
            rdfs:subClassOf prov:Association ;
            rdfs:subClassOf [
                rdf:type owl:Restriction ;
                owl:hasValue proji:Leader ;
                owl:onProperty prov:hadRole ;
              ] ;
          ] ;
        rdfs:subPropertyOf prov:qualifiedAssociation ;
      ]
      prov:agent
    ) ;
.
proj:hadObjective
  rdf:type owl:AnnotationProperty ;
  rdfs:comment "Textual definition of project objective." ;
  rdfs:domain proj:Project ;
  rdfs:label "project objective" ;
.
proj:hadPlan
  rdf:type owl:ObjectProperty ;
  rdfs:domain proj:Project ;
  rdfs:label "Project plan" ;
  rdfs:range prov:Plan ;
  rdfs:subPropertyOf prov:used ;
.
proj:hadPrincipalInvestigator
  rdf:type owl:ObjectProperty ;
  rdfs:comment "The name and label of this property are phrased retrospectively (had, was) which is consistent with PROV-O, but may be used for a contemporary relationship (has, is) while the project is underway." ;
  rdfs:domain proj:ResearchProject ;
  rdfs:label "principal investigator" ;
  rdfs:subPropertyOf proj:hadLeader ;
.
proj:hadRelatedActivity
  rdf:type owl:ObjectProperty ;
  rdfs:comment """Relationship from an activity to a related activity.

This is more general than prov:qualifiedCommunication since it is not predicated on the exchange of an entity. """ ;
  rdfs:comment "The name and label of this property are phrased retrospectively (had, was) which is consistent with PROV-O, but may be used for a contemporary relationship (has, is) while the project is underway." ;
  rdfs:domain prov:Activity ;
  rdfs:label "has related activity" ;
  rdfs:range prov:ActivityInfluence ;
  rdfs:subPropertyOf prov:qualifiedInfluence ;
  owl:inverseOf prov:activity ;
.
proj:hadSponsor
  rdf:type owl:ObjectProperty ;
  rdfs:comment "The name and label of this property are phrased retrospectively (had, was) which is consistent with PROV-O, but may be used for a contemporary relationship (has, is) while the project is underway." ;
  rdfs:domain proj:Project ;
  rdfs:label "activity sponsor" ;
  rdfs:subPropertyOf prov:wasAssociatedWith ;
  owl:propertyChainAxiom (
      [
        rdf:type owl:ObjectProperty ;
        rdfs:range [
            rdf:type owl:Class ;
            rdfs:subClassOf prov:Association ;
            rdfs:subClassOf [
                rdf:type owl:Restriction ;
                owl:hasValue proji:Sponsor ;
                owl:onProperty prov:hadRole ;
              ] ;
          ] ;
        rdfs:subPropertyOf prov:qualifiedAssociation ;
      ]
      prov:agent
    ) ;
.
proj:hadSubActivity
  rdf:type owl:ObjectProperty ;
  rdfs:comment "Relationship from an activity to a subsidiary activity." ;
  rdfs:comment "The name and label of this property are phrased retrospectively (had, was) which is consistent with PROV-O, but may be used for a contemporary relationship (has, is) while the project is underway." ;
  rdfs:domain prov:Activity ;
  rdfs:label "has sub-activity" ;
  rdfs:range prov:Activity ;
  skos:editorialNote "This property is more general than prov:wasInformedBy since it is not predicated on the exchange of an entity. " ;
.
proj:moneyAmount
  rdf:type owl:DatatypeProperty ;
  rdfs:comment "Numeric value of a sum of money, which must be scaled by a specified currency to get the actual value" ;
  rdfs:domain proj:SumOfMoney ;
  rdfs:label "Money amount" ;
  rdfs:range xsd:decimal ;
.
proj:moneyCurrency
  rdf:type owl:ObjectProperty ;
  rdfs:domain proj:SumOfMoney ;
  rdfs:label "currency of a sum of money" ;
.
proj:plannedEndTime
  rdf:type owl:DatatypeProperty ;
  rdfs:comment "The time at which an activity was planned to end. See also project:plannedStartTime."@en ;
  rdfs:domain prov:Activity ;
  rdfs:label "planned end-time" ;
  rdfs:range xsd:dateTime ;
.
proj:plannedStartTime
  rdf:type owl:DatatypeProperty ;
  rdfs:comment "The time at which an activity was planned to start. See also project:plannedEndTime."@en ;
  rdfs:domain prov:Activity ;
  rdfs:label "planned start-time" ;
  rdfs:range xsd:dateTime ;
.
proj:wasFundedThrough
  rdf:type owl:ObjectProperty ;
  rdfs:comment "The name and label of this property are phrased retrospectively (had, was) which is consistent with PROV-O, but may be used for a contemporary relationship (has, is) while the project is underway." ;
  rdfs:domain proj:Project ;
  rdfs:label "had funding association" ;
  rdfs:range proj:FundingAssociation ;
  rdfs:subPropertyOf [
      rdf:type owl:ObjectProperty ;
      rdfs:range [
          rdf:type owl:Class ;
          rdfs:subClassOf prov:Association ;
          rdfs:subClassOf [
              rdf:type owl:Restriction ;
              owl:hasValue proji:Sponsor ;
              owl:onProperty prov:hadRole ;
            ] ;
        ] ;
      rdfs:subPropertyOf prov:qualifiedAssociation ;
    ] ;
.
proj:wasSubActivityOf
  rdf:type owl:ObjectProperty ;
  rdfs:comment "Relationship from an activity to its parent activity or project." ;
  rdfs:comment "The name and label of this property are phrased retrospectively (had, was) which is consistent with PROV-O, but may be used for a contemporary relationship (has, is) while the project is underway." ;
  rdfs:label "is sub-activity of" ;
  rdfs:subPropertyOf prov:wasInformedBy ;
  owl:inverseOf proj:hasSubActivity ;
.
proji:Funder
  rdf:type prov:Role ;
  rdfs:label "funding agent role" ;
  skos:broader proji:Sponsor ;
.
proji:Leader
  rdf:type prov:Role ;
  rdfs:label "activity leader role" ;
  skos:broader proji:Participant ;
  skos:narrower proji:PrincipalInvestigator ;
.
proji:Participant
  rdf:type prov:Role ;
  rdfs:label "activity participant role" ;
.
proji:PrincipalInvestigator
  rdf:type prov:Role ;
  rdfs:label "principal investigator role" ;
  skos:broader proji:Leader ;
.
proji:Sponsor
  rdf:type prov:Role ;
  rdfs:label "sponsor role" ;
  skos:narrower proji:Funder ;
.
proji:SubActivity
  rdf:type prov:Role ;
  rdfs:label "sub-activity" ;
.
prov:Role
  rdfs:subClassOf skos:Concept ;
.
